hvhdl/ValidSS.v
@@ -11,35 +11,35 @@ Import NatMap.
 (** Defines the validss predicate that states the well-formedness and
     well-typedness of sequential statements in an H-VHDL program. *)
 
-Inductive validss (ed : ElDesign) (dstate : DState) (lenv : LEnv) : ss -> Prop :=
+Inductive validss (Δ : ElDesign) (σ : DState) (Λ : LEnv) : ss -> Prop :=
 
 (** Well-typedness of a value assignment to a declared signal. *)
 | ValidSsSigAssignDecl :
     forall {id e v t},
 
       (* Premises *)
-      vexpr ed dstate lenv false e v ->
+      vexpr Δ σ Λ false e v ->
       is_of_type v t ->
 
       (* Side conditions *)
-      MapsTo id (Declared t) ed -> (* id ∈ Sigs(Δ) and Δ(id) = t *)
+      MapsTo id (Declared t) Δ -> (* id ∈ Sigs(Δ) and Δ(id) = t *)
 
       (* Conclusion *)
-      validss ed dstate lenv (ss_sig (n_id id) e)
+      validss Δ σ Λ (ss_sig (n_id id) e)
               
 (** Well-typedness of a value assignment to a port in "out" mode. *)
 | ValidSsSigAssignOut :
     forall {id e v t},
 
       (* Premises *)
-      vexpr ed dstate lenv false e v ->
+      vexpr Δ σ Λ false e v ->
       is_of_type v t ->
 
       (* Side conditions *)
-      MapsTo id (Output t) ed -> (* id ∈ Outs(Δ) and Δ(id) = t *)
+      MapsTo id (Output t) Δ -> (* id ∈ Outs(Δ) and Δ(id) = t *)
 
       (* Conclusion *)
-      validss ed dstate lenv (ss_sig (n_id id) e)
+      validss Δ σ Λ (ss_sig (n_id id) e)
 
 (** Well-typedness of a value assignment to a declared signal
     identifier with index. *)
@@ -47,16 +47,16 @@ Inductive validss (ed : ElDesign) (dstate : DState) (lenv : LEnv) : ss -> Prop :
     forall {id e ei v vi t l u},
 
       (* Premises *)
-      vexpr ed dstate lenv false e v ->
-      vexpr ed dstate lenv false ei vi ->
+      vexpr Δ σ Λ false e v ->
+      vexpr Δ σ Λ false ei vi ->
       is_of_type v t ->
       is_of_type vi (Tnat l u) ->
                  
       (* Side conditions *)
-      MapsTo id (Declared (Tarray t l u)) ed -> (* id ∈ Sigs(Δ) and Δ(id) = array(t, l, u) *)
+      MapsTo id (Declared (Tarray t l u)) Δ -> (* id ∈ Sigs(Δ) and Δ(id) = array(t, l, u) *)
 
       (* Conclusion *)
-      validss ed dstate lenv (ss_sig (n_xid id ei) e)
+      validss Δ σ Λ (ss_sig (n_xid id ei) e)
 
 (** Well-typedness of a value assignment to an "out" port
     identifier with index. *)
@@ -64,29 +64,29 @@ Inductive validss (ed : ElDesign) (dstate : DState) (lenv : LEnv) : ss -> Prop :
     forall {id e ei v vi t l u},
 
       (* Premises *)
-      vexpr ed dstate lenv false e v ->
-      vexpr ed dstate lenv false ei vi ->
+      vexpr Δ σ Λ false e v ->
+      vexpr Δ σ Λ false ei vi ->
       is_of_type v t ->
       is_of_type vi (Tnat l u) ->
       
       (* Side conditions *)
-      MapsTo id (Output (Tarray t l u)) ed -> (* id ∈ Sigs(Δ) and Δ(id) = array(t, l, u) *)
+      MapsTo id (Output (Tarray t l u)) Δ -> (* id ∈ Sigs(Δ) and Δ(id) = array(t, l, u) *)
 
       (* Conclusion *)
-      validss ed dstate lenv (ss_sig (n_xid id ei) e)
+      validss Δ σ Λ (ss_sig (n_xid id ei) e)
               
 (** Well-typedness of a variable assignment. *)
 | ValidSsVarAssign :
     forall {id e t v val},
 
       (* Premises *)
-      vexpr ed dstate lenv false e v ->
+      vexpr Δ σ Λ false e v ->
       is_of_type v t ->
             
       (* Side conditions *)
-      MapsTo id (t, val) lenv -> (* id ∈ Λ and Λ(id) = (t, val) *)
+      MapsTo id (t, val) Λ -> (* id ∈ Λ and Λ(id) = (t, val) *)
       
-      validss ed dstate lenv (ss_var (n_id id) e)
+      validss Δ σ Λ (ss_var (n_id id) e)
 
 (** Well-typedness of a variable assignment, with an indexed
     variable identifier. *)
@@ -94,41 +94,41 @@ Inductive validss (ed : ElDesign) (dstate : DState) (lenv : LEnv) : ss -> Prop :
     forall {id e ei t v vi val l u},
 
       (* Premises *)
-      vexpr ed dstate lenv false e v ->
-      vexpr ed dstate lenv false ei vi ->
+      vexpr Δ σ Λ false e v ->
+      vexpr Δ σ Λ false ei vi ->
       is_of_type v t ->
       is_of_type vi (Tnat l u) ->
       
       (* Side conditions *)
-      MapsTo id (Tarray t l u, val) lenv -> (* id ∈ Λ and Λ(id) = (array(t,l,u), val) *)
+      MapsTo id (Tarray t l u, val) Λ -> (* id ∈ Λ and Λ(id) = (array(t,l,u), val) *)
 
       (* Conclusion *)
-      validss ed dstate lenv (ss_var (n_xid id ei) e)
+      validss Δ σ Λ (ss_var (n_xid id ei) e)
 
 (** Well-typedness of a simple if statement. *)
 | ValidSsIf :
     forall {e stmt v},
 
       (* Premises *)
-      vexpr ed dstate lenv false e v ->
+      vexpr Δ σ Λ false e v ->
       is_of_type v Tbool ->
-      validss ed dstate lenv stmt ->
+      validss Δ σ Λ stmt ->
       
       (* Conclusion *)
-      validss ed dstate lenv (ss_if e stmt)
+      validss Δ σ Λ (ss_if e stmt)
 
 (** Well-typedness of a if-else statement. *)
 | ValidSsIfElse :
     forall {e stmt stmt' v},
 
       (* Premises *)
-      vexpr ed dstate lenv false e v ->
+      vexpr Δ σ Λ false e v ->
       is_of_type v Tbool ->
-      validss ed dstate lenv stmt ->
-      validss ed dstate lenv stmt' ->
+      validss Δ σ Λ stmt ->
+      validss Δ σ Λ stmt' ->
       
       (* Conclusion *)
-      validss ed dstate lenv (ss_ifelse e stmt stmt')
+      validss Δ σ Λ (ss_ifelse e stmt stmt')
 
 (** Well-typedness of a loop statement. *)
 | ValidSsLoop :
@@ -139,28 +139,38 @@ Inductive validss (ed : ElDesign) (dstate : DState) (lenv : LEnv) : ss -> Prop :
       (** If [vexpr] interprets [e] and [e'] into [nat] values then it
          implies [is_of_type (Vnat n) nat(0,NATMAX)] and [is_of_type
          (Vnat n') nat(0,NATMAX)].  *)
-      vexpr ed dstate lenv false e (Vnat n) ->
-      vexpr ed dstate lenv false e' (Vnat n') ->
-      validss ed dstate lenv' stmt ->
+      vexpr Δ σ Λ false e (Vnat n) ->
+      vexpr Δ σ Λ false e' (Vnat n') ->
+      validss Δ σ lenv' stmt ->
       
       (* Side conditions *)
 
       (* The loop variable is added to the local environment 
          before checking the validity of the loop block statement.
        *)
-      lenv' = add id (Tnat n n', Vnat n) lenv ->
+      lenv' = add id (Tnat n n', Vnat n) Λ ->
       
       (* Conclusion *)
-      validss ed dstate lenv (ss_loop id e e' stmt)
+      validss Δ σ Λ (ss_loop id e e' stmt)
 
 (** Well-typedness of a rising edge block statement. *)
 | ValidSsRising :
     forall {stmt},
-      validss ed dstate lenv stmt ->
-      validss ed dstate lenv (ss_rising stmt)
+      validss Δ σ Λ stmt ->
+      validss Δ σ Λ (ss_rising stmt)
 
 (** Well-typedness of a falling edge block statement. *)
 | ValidSsFalling :
     forall {stmt},
-      validss ed dstate lenv stmt ->
-      validss ed dstate lenv (ss_falling stmt).
+      validss Δ σ Λ stmt ->
+      validss Δ σ Λ (ss_falling stmt)
+
+(** Well-typedness of a rst block statement *)              
+| ValidSsRst :
+    forall stmt stmt',
+      validss Δ σ Λ stmt ->
+      validss Δ σ Λ stmt' ->
+      validss Δ σ Λ (ss_rst stmt stmt')
+
+(** Well-typedness of a null statement *)
+| ValidSsNull : validss Δ σ Λ ss_null.
